stub out inline<-->tlang passes

deps/poulet4/lib/TLang/TLang.v
@@ -3,6 +3,12 @@ From Ceres Require Import Ceres.
 From Poulet4 Require Import Monads.Monad.
 From Poulet4 Require Monads.Result.
 Module R := Result.
+Import R.ResultNotations.
+Import ListNotations.
+Local Open Scope string_scope.
+Local Open Scope sexp_scope.
+From Poulet4 Require GCL.Inline.
+Module E := AST.Expr.
 
 (* This file defines the Coq version of the AST used in Egg for
    rewriting. See deps/table_opt/src/table_lang.rs for that.
@@ -14,28 +20,31 @@ Module R := Result.
 
 Inductive tm : Type :=
 | TBool (b : bool)
+| TInt (width : N) (val : Z)
 | TIf (e1 c1 c2 : tm)
 | TAnd (e1 e2 : tm)
 | TNot (e1 : tm)
-| TSet (x c : tm)
+| TSeq (c1 c2 : tm)
+| TNop
+| TSet (x e : tm)
 | TEq (x1 x2 : tm)
 | TVar (s: string)
 .
-
-Import ListNotations.
-Local Open Scope string_scope.
-Local Open Scope sexp_scope.
 (* These sexp serializers and deserializers were implemented using the
    Ceres library following this tutorial:
      https://lysxia.github.io/coq-ceres/Tutorial.html
  *)
+
 Instance Serialize_tm : Serialize tm :=
   fix sz (t : tm) : sexp :=
     match t with
     | TBool b => to_sexp b
-    | TIf e1 c1 c2 => List [Atom "if"; sz c1; sz c2]
+    | TInt w v => [Atom "int"; to_sexp w; to_sexp v]
+    | TIf e1 c1 c2 => [Atom "if"; sz c1; sz c2]
     | TAnd e1 e2 => [Atom "and"; sz e1; sz e2]
     | TNot e1 => [Atom "not"; sz e1]
+    | TSeq c1 c2 => [Atom "seq"; sz c1; sz c2]
+    | TNop => Atom "nop"
     | TSet x c => [Atom "set"; sz x; sz c]
     | TEq x1 x2 => [Atom "eq"; sz x1; sz x2]
     | TVar x => [Atom "var"; to_sexp x]
@@ -44,12 +53,13 @@ Instance Serialize_tm : Serialize tm :=
 Instance Deserialize_tm : Deserialize tm :=
   fix ds (l : loc) (e : sexp) : error + tm :=
     Deser.match_con
-      "tm" []
+      "tm" [("nop", TNop)]
       [("if",  Deser.con3 TIf ds ds ds);
        ("and", Deser.con2 TAnd ds ds);
        ("not", Deser.con1 TNot ds);
        ("set", Deser.con2 TSet ds ds);
        ("eq",  Deser.con2 TEq ds ds);
+       ("seq",  Deser.con2 TSeq ds ds);
        ("not", Deser.con1 TNot ds);
        ("var", Deser.con1_ TVar)]
       l e.
@@ -59,14 +69,90 @@ Section Optimizer.
      string (sexp). In extraction, filled in with a call to the
      table_opt Egg rewriter. *)
   Variable (ExternalOptimizer : string -> string).
+  Variable (tags_t : Type).
 
-  Definition to_string (t : tm) : string :=
+  Definition tm_to_string (t : tm) : string :=
     to_string t.
 
-  Definition from_string (s : string) : R.result error tm :=
+  Definition tm_from_string (s : string) : R.result error tm :=
     R.from_sum (from_string s).
 
-  Definition optimize (t: tm) : R.result error tm :=
-    from_string (ExternalOptimizer (to_string t)).
+  Definition optimize_tm (t: tm) : R.result error tm :=
+    tm_from_string (ExternalOptimizer (to_string t)).
+
+  Fixpoint e_to_tm (e: E.e tags_t) : R.result string tm :=
+    match e with
+    | E.EBool b _     => mret (TBool b)
+    | E.EBit w n _    => mret (TInt w n)
+    | E.EInt w n _    => mret (TInt (Npos w) n)
+    | E.EVar _ name _ => mret (TVar name)
+    | _               => R.error "e_to_tm: unimplemented"
+    end.
+
+  Fixpoint t_to_tm (stmt: Inline.t tags_t) : R.result string tm :=
+    match stmt with
+    | Inline.ISkip _ i =>
+        mret TNop
+    | Inline.IVardecl _ type x i =>
+        mret TNop
+    | Inline.IAssign _ type lhs rhs i =>
+        match lhs with
+        | AST.Expr.EVar _ name _ =>
+            let* rhs_tm := e_to_tm rhs in
+            mret (TSet (TVar name) rhs_tm)
+        | _ => mret TNop
+        end
+    | Inline.IConditional _ _ e s1 s2 _ =>
+        let* t1 := t_to_tm s1 in
+        let* t2 := t_to_tm s2 in
+        let+ e := e_to_tm e in
+        TIf e t1 t2
+    | Inline.ISeq _ s1 s2 i =>
+        let* t1 := t_to_tm s1 in
+        let+ t2 := t_to_tm s2 in
+        TSeq t1 t2
+    | Inline.IBlock _ blk =>
+        (* this breaks scope, so we need to require the original
+           stmt to have unique variable names somehow.
+
+           Better yet, statically allocate everything so that
+           IBlocks do not appear at the statement level. *)
+        t_to_tm blk
+    | Inline.IReturnVoid _ _
+    | Inline.IReturnFruit _ _ _ _
+    | Inline.IExit _ _ =>
+        (* Not sure what to do about return/etc in this setup.
+           If I have ---[x>0]--[x:=2]--+--[x:=x+1]---
+                          |            |
+                          +----[ret]---+,
+           then in P4 this is not the same as
+                     ---[x>0]--[x:=2]--+--[x:=x+1]---
+                          |
+                          +----[ret]------[x:=x+1],
+           but if ret is taken to be a primitive action, in KA,
+           they're equal.
+         *)
+        R.error "t_to_tm: exit/return unimplemented"
+    | Inline.IInvoke _ x keys actions i =>
+        R.error "t_to_tm: table invocation unimplemented"
+    | Inline.ISetValidity _ hdr val i =>
+        R.error "t_to_tm: header validity unimplemented"
+    | Inline.IHeaderStackOp _ hdr_stck_name typ op
+                            size i =>
+        R.error "t_to_tm: header stack ops unimplemented"
+    | Inline.IExternMethodCall _ extn method args i =>
+        R.error "t_to_tm: extern calls unimplemented"
+    end.
+
+  Fixpoint tm_to_t (e : tm) : R.result string (Inline.t tags_t).
+  Admitted.
+
+  Fixpoint tm_to_e (e : tm) : R.result string (Inline.t tags_t).
+  Admitted.
+
+  Definition optimize_inline_t (t: Inline.t tags_t) : R.result string (Inline.t tags_t) :=
+    let* tprog := t_to_tm t in
+    let* tprog_better := R.emap (fun x => "") (optimize_tm tprog) in
+    tm_to_t tprog_better.
 
 End Optimizer.
